commit

MergeSort.dfy
@@ -73,7 +73,7 @@ lemma LemmaS2 (a: array<int>)
 method Assign3Split(a: array<int>, middle: nat) returns (left: array<int>, right: array<int>) 
 	requires a.Length >= 2 && middle == a.Length / 2 && 0 < middle < a.Length
 	ensures forall j :: 0 <= j < middle + 1 < left.Length ==> left[j] == a[j]
-	ensures forall j :: 0 <= j < middle + 1  ==> right[j] == a[j + (middle + 1)]
+	ensures forall j :: 0 <= j < (a.Length - (middle + 1)) < right.Length  ==> right[j] == a[j + (middle + 1)]
 {
 	left := Assign3Left(a, middle);
 	right :=  Assign3Right(a, middle);
@@ -92,7 +92,7 @@ method Assign3Left(a: array<int>, middle: nat) returns (arr: array<int>)
 		// I is increasing by one
 		// arr[i] = a[i]
 		LeftLoopBody(arr, a, i, middle);
-		LemmaI(arr, a, i+1);
+		LemmaI1(arr, a, i+1, middle);
 		i := i + 1;
 	}
 } 
@@ -101,28 +101,31 @@ method LeftLoopBody(arr: array<int>, a: array<int>, i: nat, middle: nat)
 	requires a.Length >= 2 && middle == a.Length / 2 && middle > 0 // Pre
 	requires arr.Length == middle + 1
 	requires i < middle + 1 && forall j :: 0 <= j < i < arr.Length ==> arr[j] == a[j]
-	ensures forall j :: 0 <= j < i + 1 < arr.Length ==> arr[j] == a[j]
+	ensures forall j :: 0 <= j <= i  < arr.Length ==> arr[j] == a[j]
 	modifies arr
 {
-	// LemmaArrI(arr, a, i, middle);
+	LemmaArrI(arr, a, i, middle, a[i]);
 	arr[i] := a[i];
 } 
 
-lemma  LemmaArrI(arr: array<int>, a: array<int>, i: nat, middle: nat)
+lemma  LemmaArrI(arr: array<int>, a: array<int>, i: nat, middle: nat, ai: int)
 	requires a.Length >= 2 && middle == a.Length / 2 && middle > 0 // Pre
-	requires 0 <= i < middle + 1  && forall j :: 0 <= j < i < arr.Length < a.Length ==> arr[j] == a[j]
-	ensures forall j :: 0 <= j < i + 1 < arr.Length ==> arr[j] == a[j]
-{
-}
+	requires arr.Length == middle + 1 >= 2
+	requires i < middle + 1 && forall j :: 0 <= j < i < arr.Length ==> arr[j] == a[j]
+	requires ai == a[i]
+	ensures arr[..i] + [ai] == a[..i+1]
+{}
 
-lemma LemmaI (arr: array<int>, a: array<int>, i: nat)
-	requires forall j :: 0 <= j < i < arr.Length < a.Length ==> arr[j] == a[j]
+lemma LemmaI1 (arr: array<int>, a: array<int>, i: nat, middle: nat)
+	requires a.Length >= 2 && middle == a.Length / 2 && 0 < middle < a.Length
+	requires arr.Length == middle + 1 && i-1 < middle + 1
+	requires forall j :: 0 <= j < i < arr.Length ==> arr[j] == a[j] //post of LeftLoopBody
 	ensures forall j :: 0 <= j < i < arr.Length < a.Length ==> arr[j] == a[j]
 {}
 
 method Assign3Right(a: array<int>, middle: nat) returns (arr: array<int>) 
 	requires a.Length >= 2 && middle == a.Length / 2 && 0 < middle < a.Length
-	ensures forall j :: 0 <= j < middle + 1  ==> arr[j] == a[j + (middle + 1)]
+	ensures forall j :: 0 <= j < (a.Length - (middle + 1)) < arr.Length  ==> arr[j] == a[j + (middle + 1)]
 {
 	var i := 0;
 	arr := new int[a.Length - (middle + 1)];
@@ -133,39 +136,37 @@ method Assign3Right(a: array<int>, middle: nat) returns (arr: array<int>)
 		// I is increasing by one
 		// arr[i] = a[i]
 		RightLoopBody(arr, a, i, middle);
-		LemmaI(arr, a, i+1);
+		LemmaI2(arr, a, i+1, middle);
 		i := i + 1;
 	}
 } 
 
 method RightLoopBody(arr: array<int>, a: array<int>, i: nat, middle: nat) 
-	requires a.Length >= 2 && middle == a.Length / 2 && middle > 0 // Pre
-	requires 0 <= i < a.Length - (middle + 1) && forall j :: 0 <= j < i < arr.Length ==> arr[j] == a[j + middle + 1] // Inv // Guard
+	requires a.Length >= 2 && middle == a.Length / 2 && 0 < middle < a.Length // Pre
+	requires 0 <= i < a.Length - (middle + 1) // Guard
+	requires forall j :: 0 <= j < i < arr.Length ==> arr[j] == a[j + middle + 1] // Inv
 	requires arr.Length == a.Length - (middle + 1)
 	ensures forall j :: 0 <= j <= i < arr.Length ==> arr[j] == a[j + middle + 1]
 	modifies arr
 {
-	LemmaArrIRight(arr, a, i, middle, a[i]);
-	assert a.Length - (middle + 1) < a.Length;
-	arr[i] := a[i];
+	LemmaArrIRight(arr, a, i, middle, a[i + middle + 1]);
+	arr[i] := a[i + middle + 1];
 } 
 
 lemma LemmaArrIRight(arr: array<int>, a: array<int>, i: nat, middle: nat, ai: int)
-	requires a.Length >= 2 && middle == a.Length / 2 && middle > 0 // Pre
-	requires i < a.Length - (middle + 1) // Guard
+	requires a.Length >= 2 && middle == a.Length / 2 && 0 < middle < a.Length // Pre
+	requires 0 <= i < a.Length - (middle + 1) // Guard
+	requires ai == a[i + middle + 1] && arr.Length == a.Length - (middle + 1)
 	requires forall j :: 0 <= j < i < arr.Length ==> arr[j] == a[j + middle + 1] // Inv
-	ensures forall j :: 0 <= j < i < arr.Length ==> arr[j] == a[j + middle + 1] && a[i] == a[i]
-{
-	// Strengthen Post Condition
-}
+	ensures arr[..i] + [ai] == a[middle+1 .. (i + middle + 2)]
+{}
 
-// lemma LemmaI (arr: array<int>, a: array<int>, i: nat)
-// 	requires arr[..i] == a[..i]
-// 	ensures arr[..i] == a[..i]
-// {}
-
-
-
+lemma LemmaI2 (arr: array<int>, a: array<int>, i: nat, middle: nat)
+	requires a.Length >= 2 && middle == a.Length / 2 && 0 < middle < a.Length
+	requires i-1 < a.Length - (middle + 1) // Guard
+	requires forall j :: 0 <= j < i < arr.Length ==> arr[j] == a[j + middle + 1] //post of RighttLoopBody
+	ensures forall j :: 0 <= j < i < arr.Length ==> arr[j] == a[j + middle + 1]
+{}
 
 
 method Merge(b: array<int>, c: array<int>, d: array<int>)
